Answer exercise 4.4.

Star.thy
@@ -7,10 +7,7 @@ inductive star :: "('a \<Rightarrow> 'a \<Rightarrow> bool) \<Rightarrow> 'a \<R
 (* By definition, star r is reflexive and transitive,
    but we need rule induction to prove: *)
 lemma star_trans: "star r x y \<Longrightarrow> star r y z \<Longrightarrow> star r x z"
-  apply (induction rule: star.induct)
-  apply (assumption)
-  apply (metis step)
-done
+by (induction rule: star.induct, assumption, metis step)
 
 (* Exercise 4.2 *)
 inductive palindrome :: "'a list \<Rightarrow> bool" where
@@ -19,5 +16,14 @@ inductive palindrome :: "'a list \<Rightarrow> bool" where
 
 theorem "palindrome xs \<Longrightarrow> (rev xs) = xs"
 by (induction xs rule: palindrome.induct, auto)
+
+(* Exercise 4.4 *)
+(* Inductive definition of the n-fold iteration of a relation [r]. *)
+inductive iter :: "('a \<Rightarrow> 'a \<Rightarrow> bool) \<Rightarrow> int \<Rightarrow> 'a \<Rightarrow> 'a \<Rightarrow> bool"  where
+  iter_refl: "iter r 0 x x"
+| iter_step: "r x y \<Longrightarrow> iter r n y z \<Longrightarrow> iter r (n + 1) x z"
+
+theorem "star r x y \<Longrightarrow> \<exists>n. iter r n x y"
+by (induction rule: star.induct, auto intro: iter_refl iter_step)
 
 end
